Proofs/AES-GCM/GCMGmultV8Sym.lean
@@ -1,6 +1,7 @@
 import Tests.«AES-GCM».GCMGmultV8Program
 import Tactics.Sym
 import Tactics.StepThms
+import Specs.GCMV8
 
 namespace GCMGmultV8Program
 
@@ -12,9 +13,32 @@ theorem gcm_gmult_v8_program_run_27 (s0 sf : ArmState)
     (h_s0_pc : read_pc s0 = gcm_gmult_v8_program.min)
     (h_s0_sp_aligned : CheckSPAlignment s0)
     (h_run : sf = run gcm_gmult_v8_program.length s0) :
-    read_err sf = .None := by
+    read_err sf = .None
+    ∧ let xiAddr := r (.GPR 0#5) s0
+      let hTableAddr := r (.GPR 1#5) s0
+      let xiInput := read_mem_bytes 16 xiAddr s0
+      let hTable := read_mem_bytes (16) hTableAddr s0
+      let xiOut := read_mem_bytes 16 xiAddr sf
+      xiOut = GCMV8.GCMGmultV8' hTable xiInput
+    := by
   simp (config := {ground := true}) only at h_s0_pc
   -- ^^ Still needed, because `gcm_gmult_v8_program.min` is somehow
   --    unable to be reflected
   sym_n 27
+  conv => {
+    rhs;
+    simp [GCMV8.GCMGmultV8', GCMV8.gcm_polyval,
+      GCMV8.gcm_polyval_red,
+      GCMV8.gcm_polyval_mul,
+      GCMV8.gcm_init_H,
+      GCMV8.pmult,
+      GCMV8.pmod,
+      GCMV8.lo,
+      GCMV8.hi,
+      GCMV8.irrepoly,
+      bitvec_rules,
+      minimal_theory
+      ]
+  }
+  sorry
   done
